updates

intermediate/Veritas.Intermediate.Logs.fst
@@ -6,87 +6,87 @@ open Veritas.MultiSetHashDomain
 open Veritas.Record
 open Veritas.SeqAux
 open Veritas.State
+open Veritas.Intermediate.VerifierConfig
 
 module Spec = Veritas.Verifier
-
-let slot_id = nat
-let thread_id = Spec.thread_id
 
 (* Definitions of different styles of verifier logs.
    - logK : contains only key references (defined in Veritas.Verifier)
    - logS: contains slot references
    - logL: contains slot references & low-level data structures (TODO) *)
 
+let thread_id = Spec.thread_id
+
 let logK_entry = Spec.vlog_entry
 let logK = Spec.vlog
 
-type logS_entry =
-  | Get_S: s:slot_id -> k:data_key -> v:data_value -> logS_entry
-  | Put_S: s:slot_id -> k:data_key -> v:data_value -> logS_entry
-  | AddM_S: s:slot_id -> r:record -> s':slot_id -> logS_entry
-  | EvictM_S: s:slot_id -> s':slot_id -> logS_entry
-  | AddB_S: s:slot_id -> r:record -> t:timestamp -> j:thread_id -> logS_entry
-  | EvictB_S: s:slot_id -> t:timestamp -> logS_entry
-  | EvictBM_S: s:slot_id -> s':slot_id -> t:timestamp -> logS_entry
+type logS_entry (vcfg:verifier_config) =
+  | Get_S: s:slot_id vcfg -> k:data_key -> v:data_value -> logS_entry vcfg
+  | Put_S: s:slot_id vcfg -> k:data_key -> v:data_value -> logS_entry vcfg
+  | AddM_S: s:slot_id vcfg -> r:record -> s':slot_id vcfg -> logS_entry vcfg
+  | EvictM_S: s:slot_id vcfg -> s':slot_id vcfg -> logS_entry vcfg
+  | AddB_S: s:slot_id vcfg -> r:record -> t:timestamp -> j:thread_id -> logS_entry vcfg
+  | EvictB_S: s:slot_id vcfg -> t:timestamp -> logS_entry vcfg
+  | EvictBM_S: s:slot_id vcfg -> s':slot_id vcfg -> t:timestamp -> logS_entry vcfg
              
-let logS = Seq.seq logS_entry
+let logS vcfg = Seq.seq (logS_entry vcfg)
 
-let is_state_op (e: logS_entry): bool =
+let is_state_op #vcfg (e: logS_entry vcfg): bool =
   match e with
   | Get_S _ _ _ | Put_S _ _ _ -> true
   | _ -> false
 
-let to_state_op (e:logS_entry {is_state_op e}): state_op =
+let to_state_op #vcfg (e:logS_entry vcfg {is_state_op e}): state_op =
   match e with
   | Get_S _ k v -> Get k v
   | Put_S _ k v -> Put k v
 
-let to_state_op_logS (l: logS) =
+let to_state_op_logS #vcfg (l: logS vcfg) =
   map to_state_op (filter_refine is_state_op l)
 
 (* Reproducing definitions from Veritas.Verifier.Thread *)
 
-let thread_id_logS = thread_id & logS
+let thread_id_logS (vcfg:verifier_config) = thread_id & logS vcfg
 
-let thread_id_of (tl: thread_id_logS): nat = fst tl
+let thread_id_of #vcfg (tl: thread_id_logS vcfg): nat = fst tl
 
-let logS_of (tl: thread_id_logS): logS = snd tl
+let logS_of #vcfg (tl: thread_id_logS vcfg): logS _ = snd tl
 
-let tl_length (tl: thread_id_logS): nat =
+let tl_length #vcfg (tl: thread_id_logS vcfg): nat =
   Seq.length (logS_of tl)
 
-let tl_idx (tl: thread_id_logS) = i:nat{i < tl_length tl}
+let tl_idx #vcfg (tl: thread_id_logS vcfg) = i:nat{i < tl_length tl}
 
-let tl_index (tl: thread_id_logS) (i:tl_idx tl): logS_entry =
+let tl_index #vcfg (tl: thread_id_logS vcfg) (i:tl_idx tl): logS_entry _ =
   Seq.index (logS_of tl) i
 
-let tl_prefix (tl: thread_id_logS) (i:nat{i <= tl_length tl}): thread_id_logS =
+let tl_prefix #vcfg (tl: thread_id_logS vcfg) (i:nat{i <= tl_length tl}): thread_id_logS _ =
   (thread_id_of tl), (prefix (logS_of tl) i)
 
 (* Reproducing definitions from Veritas.Verifier.Global *)
 
-let g_logS = Seq.seq logS
+let g_logS vcfg = Seq.seq (logS vcfg)
 
-let thread_log (gl:g_logS) (tid:seq_index gl): thread_id_logS = 
+let thread_log #vcfg (gl:g_logS vcfg) (tid:seq_index gl): thread_id_logS _ = 
    (tid, Seq.index gl tid)
 
-let to_state_op_glogS (gl:g_logS) =
+let to_state_op_glogS #vcfg (gl:g_logS vcfg) =
   map to_state_op_logS gl
 
 (* Reproducing definitions from Veritas.Verifier.TSLog *)
 
-let il_logS = interleaving logS_entry
+let il_logS vcfg = interleaving (logS_entry vcfg)
 
-let thread_count (il:il_logS) = Seq.length (s_seq il)
+let thread_count #vcfg (il:il_logS vcfg) = Seq.length (s_seq il)
 
-let valid_tid (il:il_logS) = tid:nat{tid < thread_count il}
+let valid_tid #vcfg (il:il_logS vcfg) = tid:nat{tid < thread_count il}
 
-let g_logS_of (il:il_logS): g_logS = s_seq il
+let g_logS_of #vcfg (il:il_logS vcfg): g_logS _ = s_seq il
 
-let state_ops (itsl:il_logS): Seq.seq (state_op) =
+let state_ops #vcfg (itsl:il_logS vcfg): Seq.seq (state_op) =
   to_state_op_logS (i_seq itsl)
 
-let lemma_logS_interleave_implies_state_ops_interleave (l: logS) (gl: g_logS{interleave #logS_entry l gl})
+let lemma_logS_interleave_implies_state_ops_interleave #vcfg (l: logS vcfg) (gl: g_logS vcfg{interleave #(logS_entry vcfg) l gl})
   : Lemma (interleave #state_op (to_state_op_logS l) (to_state_op_glogS gl)) 
   = FStar.Squash.bind_squash
       #(interleave l gl)
