intermediate/Veritas.Intermediate.Verify.fsti
@@ -274,20 +274,18 @@ let vevictbm #vcfg (s:slot_id vcfg) (s':slot_id vcfg) (t:timestamp) (vs:vtls vcf
             let st_upd = mevict_from_store st_upd s s' d in
             update_thread_store vs st_upd
 
-(*
-
 (* Relation between thread-local states
    * either both states have Failed
    * or both are Valid with equal contents
      (note that store_rel st st' enforces is_map st) *)
-let vtls_rel (vs:vtls) (vs':Spec.vtls) : Type =
+let vtls_rel #vcfg (vs:vtls vcfg) (vs':Spec.vtls) : Type =
   (Failed? vs /\ Spec.Failed? vs') \/
   (Valid? vs /\ Spec.Valid? vs' /\
    (let Valid id st clk ha he = vs in
     let Spec.Valid id' st' clk' _ ha' he' = vs' in
     store_rel st st' /\ id = id' /\ clk = clk' /\ ha = ha' /\ he = he'))
 
-let t_verify_step (vs:vtls) (e:logS_entry): vtls =
+let t_verify_step #vcfg (vs:vtls vcfg) (e:logS_entry vcfg): vtls vcfg =
   match vs with
   | Failed -> Failed
   | _ ->
@@ -303,38 +301,38 @@ let t_verify_step (vs:vtls) (e:logS_entry): vtls =
 (* Convert slot-based log entry e to a key-based log entry, given verifier state vs.
    This is basically a "light" version of the vfun functions that reconstructs the log. 
    We could have the vfun functions return logK entries instead, but this seems cleaner. *)
-let logS_to_logK_entry (vs:vtls{Valid? vs}) (e:logS_entry) : option logK_entry =
+let logS_to_logK_entry #vcfg (vs:vtls vcfg {Valid? vs}) (e:logS_entry vcfg) : option logK_entry =
   let st = thread_store vs in
   match e with
   | Get_S s k v -> 
-      if store_contains st s && k = stored_key st s
+      if inuse_slot st s && k = stored_key st s
       then Some (Spec.Get k v) else None
   | Put_S s k v -> 
-      if store_contains st s && k = stored_key st s
+      if inuse_slot st s && k = stored_key st s
       then Some (Spec.Put k v) else None
   | AddM_S _ r s' -> 
-      if store_contains st s' && is_merkle_key (stored_key st s') 
+      if inuse_slot st s' && is_merkle_key (stored_key st s') 
       then Some (Spec.AddM r (stored_key st s')) else None
   | EvictM_S s s' -> 
-      if store_contains st s && store_contains st s' && is_merkle_key (stored_key st s') 
+      if inuse_slot st s && inuse_slot st s' && is_merkle_key (stored_key st s') 
       then Some (Spec.EvictM (stored_key st s) (stored_key st s')) else None
   | AddB_S _ r t j -> 
       Some (Spec.AddB r t j)
   | EvictB_S s t -> 
-      if store_contains st s
+      if inuse_slot st s
       then Some (Spec.EvictB (stored_key st s) t) else None
   | EvictBM_S s s' t ->
-      if store_contains st s && store_contains st s' && is_merkle_key (stored_key st s') 
+      if inuse_slot st s && inuse_slot st s' && is_merkle_key (stored_key st s') 
       then Some (Spec.EvictBM (stored_key st s) (stored_key st s') t) else None
 
 (* Add the logK_entry equivalent of e to log l, given current state vs. *)
-let add_to_log (l:option logK) (vs:vtls) (e:logS_entry) : option logK =
+let add_to_log #vcfg (l:option logK) (vs:vtls vcfg) (e:logS_entry vcfg) : option logK =
   if Some? l && Valid? vs && Some? (logS_to_logK_entry vs e)
   then Some (append1 (Some?.v l) (Some?.v (logS_to_logK_entry vs e)))
   else None
 
 (* Verify a log from a specified initial state. *)
-let rec t_verify_aux (vs:vtls) (l:logS): Tot (vtls * option logK)
+let rec t_verify_aux #vcfg (vs:vtls vcfg) (l:logS vcfg): Tot ((vtls vcfg) * option logK)
   (decreases (Seq.length l)) =
   let n = Seq.length l in
   if n = 0 then (vs, Some Seq.empty)
@@ -346,71 +344,68 @@ let rec t_verify_aux (vs:vtls) (l:logS): Tot (vtls * option logK)
     let lk' = add_to_log lk vsp e in
     (vs', lk')
 
-val lemma_t_verify_aux_valid_implies_log_exists (vs:vtls) (l:logS)
+val lemma_t_verify_aux_valid_implies_log_exists (#vcfg:_) (vs:vtls vcfg) (l:logS vcfg)
   : Lemma (requires (Valid? (fst (t_verify_aux vs l))))
           (ensures (Some? (snd (t_verify_aux vs l))))
           (decreases (Seq.length l))
           [SMTPat (Some? (snd (t_verify_aux vs l)))]
 
-(* Initialize verifier state *)
-// TODO: what should the initial size be?
-let store_size = 65536 // 2 ^ 16
-let init_thread_state (id:thread_id): vtls = 
-  let vs = Valid id (empty_store store_size) (MkTimestamp 0 0) empty_hash_value empty_hash_value in  
+let init_thread_state #vcfg (id:thread_id): vtls vcfg = 
+  let vs = Valid id (empty_store vcfg) (MkTimestamp 0 0) empty_hash_value empty_hash_value in  
   if id = 0 then
     let st0 = thread_store vs in
-    let st0_upd = add_to_store st0 0 Root (init_value Root) Spec.MAdd in
+    let st0_upd = madd_to_store_root st0 0 (init_value Root) in
     update_thread_store vs st0_upd    
   else vs
 
 (* Main thread-level verify function *)
-let t_verify (id:thread_id) (l:logS): vtls = 
+let t_verify #vcfg (id:thread_id) (l:logS vcfg): vtls vcfg = 
   fst (t_verify_aux (init_thread_state id) l) 
 
-let logS_to_logK (id:thread_id) (l:logS{Valid? (t_verify id l)}) : logK =
-  Some?.v (snd (t_verify_aux (init_thread_state id) l))
+let logS_to_logK #vcfg (id:thread_id) (l:logS vcfg{Valid? (t_verify id l)}) : logK =
+  Some?.v (snd (t_verify_aux (init_thread_state #vcfg id) l))
 
-let init_thread_state_valid (id:thread_id)
-  : Lemma (Valid? (init_thread_state id))
-          [SMTPat (init_thread_state id)]
+let init_thread_state_valid #vcfg (id:thread_id)
+  : Lemma (Valid? (init_thread_state #vcfg id))
+          [SMTPat (init_thread_state #vcfg id)]
   = ()
 
 (** Utilities for running a single verifier thread.
     Follows the definitions in Veritas.Verifier.Thread. **)
 
-let verify (tl:thread_id_logS): vtls =
+let verify #vcfg (tl:thread_id_logS vcfg): vtls _ =
   t_verify (fst tl) (snd tl)
-  
-let tl_verifiable (tl: thread_id_logS): bool =
+
+let tl_verifiable #vcfg (tl: thread_id_logS vcfg): bool =
   Valid? (verify tl)
 
-let tl_verifiable_log = tl: thread_id_logS {tl_verifiable tl}
+let tl_verifiable_log #vcfg = tl: thread_id_logS vcfg {tl_verifiable tl}
 
 val lemma_tl_verifiable_implies_prefix_verifiable
-  (tl:tl_verifiable_log) (i:nat{i <= tl_length tl}):
+  (#vcfg:_) (tl:tl_verifiable_log #vcfg) (i:nat{i <= tl_length tl}):
   Lemma (ensures (tl_verifiable (tl_prefix tl i)))
-        [SMTPat (tl_prefix tl i)]
 
-let tl_clock (tl:tl_verifiable_log) (i:tl_idx tl): timestamp =
-  Valid?.clock (verify (tl_prefix tl (i + 1)))
+let tl_clock #vcfg (tl:tl_verifiable_log #vcfg) (i:tl_idx tl): timestamp =
+  let vs = verify #vcfg (tl_prefix tl (i + 1)) in
+  lemma_tl_verifiable_implies_prefix_verifiable tl (i + 1);
+  Valid?.clock (verify #vcfg (tl_prefix tl (i + 1)))
 
-let tl_verify (tl:thread_id_logS) (i:tl_idx tl): vtls =
+let tl_verify #vcfg (tl:thread_id_logS vcfg) (i:tl_idx tl): vtls _ =
   verify (tl_prefix tl (i + 1))
 
 (* Utilities for running all verifier threads and comparing aggregate add/evict hashes.
    Follows the definitions in Veritas.Verifier.Global. *) 
-
-let gl_verifiable (gl: g_logS) = 
+let gl_verifiable #vcfg (gl: g_logS vcfg) = 
   forall (tid:seq_index gl). tl_verifiable (thread_log gl tid)
 
-let gl_verifiable_log = gl:g_logS{gl_verifiable gl}
+let gl_verifiable_log vcfg = gl:g_logS vcfg{gl_verifiable gl}
 
 val lemma_gl_verifiable_implies_prefix_verifiable
-  (gl:gl_verifiable_log) (i:nat{i <= Seq.length gl}):
-  Lemma (ensures (gl_verifiable (prefix gl i)))
+  (#vcfg:_) (gl:gl_verifiable_log vcfg) (i:nat{i <= Seq.length gl}):
+  Lemma (ensures (gl_verifiable #vcfg (prefix gl i)))
         [SMTPat (prefix gl i)]
 
-let rec hadd_aux (gl: gl_verifiable_log)
+let rec hadd_aux #vcfg (gl: gl_verifiable_log vcfg)
   : Tot (ms_hash_value)
     (decreases (Seq.length gl)) 
   = let p = Seq.length gl in
@@ -421,9 +416,9 @@ let rec hadd_aux (gl: gl_verifiable_log)
       let h2 = thread_hadd (verify (thread_log gl (p - 1))) in
       ms_hashfn_agg h1 h2
 
-let hadd (gl: gl_verifiable_log): ms_hash_value = hadd_aux gl
+let hadd #vcfg (gl: gl_verifiable_log vcfg): ms_hash_value = hadd_aux gl
 
-let rec hevict_aux (gl: gl_verifiable_log)
+let rec hevict_aux #vcfg (gl: gl_verifiable_log vcfg)
   : Tot (ms_hash_value)
     (decreases (Seq.length gl))
   = let p = Seq.length gl in
@@ -434,19 +429,19 @@ let rec hevict_aux (gl: gl_verifiable_log)
       let h2 = thread_hevict (verify (thread_log gl (p - 1))) in
       ms_hashfn_agg h1 h2
 
-let hevict (gl: gl_verifiable_log): ms_hash_value = hevict_aux gl
+let hevict #vcfg (gl: gl_verifiable_log vcfg): ms_hash_value = hevict_aux gl
 
-let gl_hash_verifiable (gl: gl_verifiable_log): bool = 
+let gl_hash_verifiable #vcfg (gl: gl_verifiable_log vcfg): bool = 
   hadd gl = hevict gl
 
-let gl_hash_verifiable_log = gl:gl_verifiable_log{gl_hash_verifiable gl}
+let gl_hash_verifiable_log vcfg = gl:gl_verifiable_log vcfg{gl_hash_verifiable gl}
 
-let gl_clock (gl:gl_verifiable_log) (i:I.sseq_index gl): timestamp = 
+let gl_clock #vcfg (gl:gl_verifiable_log vcfg) (i:I.sseq_index gl): timestamp = 
   let (tid, idx) = i in  
   let tl = thread_log gl tid in
   tl_clock tl idx
 
-let gl_verify (gl:g_logS) (i:I.sseq_index gl): vtls =
+let gl_verify #vcfg (gl:g_logS vcfg) (i:I.sseq_index gl): vtls _ =
   let (tid, idx) = i in  
   let tl = thread_log gl tid in
   tl_verify tl idx
@@ -454,34 +449,33 @@ let gl_verify (gl:g_logS) (i:I.sseq_index gl): vtls =
 (* Utilities for verifying the global, interleaved log shared among all threads.
    Follows the definitions in Veritas.Verifier.TSLog. *) 
 
-let il_verifiable (il: il_logS) = 
+let il_verifiable #vcfg (il: il_logS vcfg) = 
   gl_verifiable (g_logS_of il)
 
-let il_clock (il: il_logS{il_verifiable il}) (i: I.seq_index il): timestamp =
+let il_clock #vcfg (il: il_logS vcfg{il_verifiable il}) (i: I.seq_index il): timestamp =
   let gl = g_logS_of il in
   let j = I.i2s_map il i in
   gl_clock gl j
 
 (* state at thread j after processing log entry i (which modifies the state of j) *)
-let il_verify (il: il_logS) (i: I.seq_index il): vtls =
+let il_verify #vcfg (il: il_logS vcfg) (i: I.seq_index il): vtls _ =
   let gl = g_logS_of il in
   let j = I.i2s_map il i in
   gl_verify gl j
 
-val clock_sorted (il: il_logS {il_verifiable il}): prop
- 
-let its_log = il:il_logS{il_verifiable il /\ clock_sorted il}
+val clock_sorted (#vcfg:_) (il: il_logS vcfg {il_verifiable il}): prop
 
-let il_hash_verifiable (itsl: its_log) = gl_hash_verifiable (g_logS_of itsl)
+let its_log vcfg = il:il_logS vcfg{il_verifiable il /\ clock_sorted il}
 
-let il_hash_verifiable_log = itsl:its_log {il_hash_verifiable itsl}
+let il_hash_verifiable #vcfg (itsl: its_log vcfg) = gl_hash_verifiable (g_logS_of itsl)
 
-val lemma_prefix_verifiable (itsl: its_log) (i:nat{i <= I.length itsl}):
+let il_hash_verifiable_log vcfg = itsl:its_log vcfg{il_hash_verifiable itsl}
+
+val lemma_prefix_verifiable (#vcfg:_) (itsl: its_log vcfg) (i:nat{i <= I.length itsl}):
   Lemma (ensures (il_verifiable (I.prefix itsl i) /\ clock_sorted (I.prefix itsl i)))
         [SMTPat (I.prefix itsl i)]
 
 // final correctness property
-val lemma_verifier_correct (gl: gl_hash_verifiable_log { ~ (seq_consistent (to_state_op_glogS gl))})
+val lemma_verifier_correct (#vcfg:_) (gl: gl_hash_verifiable_log vcfg { ~ (seq_consistent (to_state_op_glogS gl))})
   : hash_collision_gen 
-*)
 
